Simplify weakest precondition and make it plain

theories/pure_program_logic/weakestpre.v
@@ -1,50 +1,40 @@
-From iris.base_logic.lib Require Export fancy_updates.
+From iris.base_logic Require Export iprop.
 From iris.program_logic Require Export language.
 From iris.bi Require Export weakestpre.
 From iris.proofmode Require Import base tactics classes.
+
+From D.iris_extra Require Export det_reduction.
 Set Default Proof Using "Type".
 Import uPred.
 
-(* The following development is that of a *Plain* weakest
-precondition. In the sense that it does not require any  *)
+(*
+The following development is that of a *Plain* weakest
+precondition: it uses no (basic/fancy) updates, does not supports Iris invariants,
+and is specialized to deterministic languages.
+*)
 
 Class irisG (Λ : language) (Σ : gFunctors) := IrisG {
-
-  (** The state interpretation is an invariant that should hold in between each
-  step of reduction. Here [Λstate] is the global state, [list Λobservation] are
-  the remaining observations, and [nat] is the number of forked-off threads
-  (not the total number of threads, which is one higher because there is always
-  a main thread). *)
-  state_interp : state Λ → list (observation Λ) → nat → iProp Σ;
-
-  (** A fixed postcondition for any forked-off thread. For most languages, e.g.
-  heap_lang, this will simply be [True]. However, it is useful if one wants to
-  keep track of resources precisely, as in e.g. Iron. *)
-  fork_post : val Λ → iProp Σ;
+  irisG_langdet :> LangDet Λ
 }.
+Arguments IrisG {_ _} _.
+Local Notation σ := dummyState.
 
-Definition wp_pre `{irisG Λ Σ} (s : stuckness)
-    (wp : coPset -d> expr Λ -d> (val Λ -d> iPropO Σ) -d> iPropO Σ) :
-    coPset -d> expr Λ -d> (val Λ -d> iPropO Σ) -d> iPropO Σ := λ E e1 Φ,
+Definition wp_pre `{irisG Λ Σ}
+    (wp : expr Λ -d> (val Λ -d> iPropO Σ) -d> iPropO Σ) :
+    expr Λ -d> (val Λ -d> iPropO Σ) -d> iPropO Σ := λ e1 Φ,
   match to_val e1 with
   | Some v => Φ v
-  | None => ∀ σ1 κ κs n,
-     state_interp σ1 (κ ++ κs) n -∗
-       ⌜if s is NotStuck then reducible e1 σ1 else True⌝ ∗
-       ∀ e2 σ2 efs, ⌜prim_step e1 σ1 κ e2 σ2 efs⌝ -∗
-          ▷ (state_interp σ2 κs (length efs + n) ∗
-         wp E e2 Φ ∗
-         [∗ list] i ↦ ef ∈ efs, wp ⊤ ef fork_post)
+  | None => ∃ e2, ⌜prim_step e1 σ [] e2 σ []⌝ ∧ ▷ wp e2 Φ
   end%I.
 
-Local Instance wp_pre_contractive `{irisG Λ Σ} s : Contractive (wp_pre s).
+Local Instance wp_pre_contractive `{irisG Λ Σ} : Contractive wp_pre.
 Proof.
-  rewrite /wp_pre=> n wp wp' Hwp E e1 Φ.
+  rewrite /wp_pre => n wp wp' Hwp e1 Φ.
   repeat (f_contractive || f_equiv); apply Hwp.
 Qed.
 
-Definition wp_def `{irisG Λ Σ} (s : stuckness) :
-  coPset → expr Λ → (val Λ → iProp Σ) → iProp Σ := fixpoint (wp_pre s).
+Definition wp_def `{irisG Λ Σ} : stuckness → coPset →
+   expr Λ → (val Λ → iProp Σ) → iProp Σ := λ _ _, fixpoint wp_pre.
 Definition wp_aux `{irisG Λ Σ} : seal (@wp_def Λ Σ _). by eexists. Qed.
 Instance wp' `{irisG Λ Σ} : Wp Λ (iProp Σ) stuckness := wp_aux.(unseal).
 Definition wp_eq `{irisG Λ Σ} : wp = @wp_def Λ Σ _ := wp_aux.(seal_eq).
@@ -59,19 +49,16 @@ Implicit Types e : expr Λ.
 
 (* Weakest pre *)
 Lemma wp_unfold s E e Φ :
-  WP e @ s; E {{ Φ }} ⊣⊢ wp_pre s (wp (PROP:=iProp Σ)  s) E e Φ.
-Proof. rewrite wp_eq. apply (fixpoint_unfold (wp_pre s)). Qed.
+  WP e @ s; E {{ Φ }} ⊣⊢ wp_pre (wp (PROP:=iProp Σ) s E) e Φ.
+Proof. rewrite wp_eq. apply (fixpoint_unfold wp_pre). Qed.
 
 Global Instance wp_ne s E e n :
   Proper (pointwise_relation _ (dist n) ==> dist n) (wp (PROP:=iProp Σ) s E e).
 Proof.
-  revert e. induction (lt_wf n) as [n _ IH]=> e Φ Ψ HΦ.
+  elim: (lt_wf n) e => {}n _ IH e Φ Ψ HΦ.
   rewrite !wp_unfold /wp_pre.
-  (* FIXME: figure out a way to properly automate this proof *)
-  (* FIXME: reflexivity, as being called many times by f_equiv and f_contractive
-  is very slow here *)
-  do 21 (f_contractive || f_equiv). apply IH; first lia.
-  intros v. eapply dist_le; eauto with lia.
+  repeat first [apply IH; first lia | f_contractive | f_equiv].
+  eapply dist_le; eauto with lia.
 Qed.
 Global Instance wp_proper s E e :
   Proper (pointwise_relation _ (≡) ==> (≡)) (wp (PROP:=iProp Σ) s E e).
@@ -85,128 +72,116 @@ Proof.
   intros He Φ Ψ HΦ. rewrite !wp_unfold /wp_pre He.
   by repeat (f_contractive || f_equiv).
 Qed.
+Global Instance wp_plain s E e Φ (HΦ: ∀ v, Plain (Φ v)):
+  Plain (wp (PROP:=iProp Σ) s E e Φ).
+Proof.
+  rewrite /Plain; iLöb as "IH" forall (e).
+  iEval rewrite !wp_unfold /wp_pre.
+  case_match; first by iApply plain.
+  iDestruct 1 as (e2 ?) "H2"; iExists e2; iSplit; first done.
+  rewrite -later_plainly; by iApply ("IH" $! e2 with "H2").
+Qed.
 
 Lemma wp_value' s E Φ v : Φ v ⊢ WP of_val v @ s; E {{ Φ }}.
 Proof. iIntros "HΦ". rewrite wp_unfold /wp_pre to_of_val. auto. Qed.
 Lemma wp_value_inv' s E Φ v : WP of_val v @ s; E {{ Φ }} ⊢ Φ v.
 Proof. by rewrite wp_unfold /wp_pre to_of_val. Qed.
 
-Lemma wp_strong_mono s1 s2 E1 E2 e Φ Ψ :
-  s1 ⊑ s2 →
-  WP e @ s1; E1 {{ Φ }} -∗ (∀ v, Φ v -∗ Ψ v) -∗ WP e @ s2; E2 {{ Ψ }}.
+Lemma wp_strong_mono e Φ Ψ :
+  WP e {{ Φ }} -∗ (∀ v, Φ v -∗ Ψ v) -∗ WP e {{ Ψ }}.
 Proof.
-  iIntros (?) "H HΦ". iLöb as "IH" forall (e E1 E2 Φ Ψ).
+  iIntros "H HΦ". iLöb as "IH" forall (e Φ Ψ).
   rewrite !wp_unfold /wp_pre.
-  destruct (to_val e) as [v|] eqn:?.
-  { by iApply ("HΦ" with "[-]"). }
-  iIntros (σ1 κ κs n) "Hσ".
-  iDestruct ("H" with "[$]") as "[% H]".
-  iSplit; [by destruct s1, s2|]. iIntros (e2 σ2 efs Hstep).
-  iDestruct ("H" with "[//]") as "H". iIntros "!>".
-  iDestruct "H" as "(Hσ & H & Hefs)".
-  iFrame "Hσ". iSplitR "Hefs".
-  - iApply ("IH" with "H HΦ").
-  - iApply (big_sepL_impl with "Hefs"); iIntros "!#" (k ef _).
-    iIntros "H". iApply ("IH" with "H"); auto.
+  destruct (to_val e) as [v|]; first by iApply ("HΦ" with "[-]").
+  iDestruct "H" as (e2 ?) "H".
+  iExists e2; iSplit; first done; iIntros "!>".
+  iApply ("IH" with "H HΦ").
 Qed.
 
-Lemma wp_step s E1 E2 e P Φ :
+Lemma wp_step e P Φ :
   to_val e = None →
-  (▷ P) -∗ WP e @ s; E2 {{ v, P -∗ Φ v }} -∗ WP e @ s; E1 {{ Φ }}.
+  (▷ P) -∗ WP e {{ v, P -∗ Φ v }} -∗ WP e {{ Φ }}.
 Proof.
-  rewrite !wp_unfold /wp_pre. iIntros (->) "HR H".
-  iIntros (σ1 κ κs n) "Hσ". iDestruct ("H" with "[$]") as "[$ H]".
-  iIntros (e2 σ2 efs Hstep). iDestruct ("H" $! e2 σ2 efs with "[% //]") as "H".
-  iIntros "!>". iDestruct "H" as "(Hσ & H & Hefs)".
-  iFrame "Hσ Hefs".
-  iApply (wp_strong_mono s s E2 with "H"); [done..|].
+  rewrite !wp_unfold /wp_pre; iIntros (->) "HR".
+  iDestruct 1 as (e2) "[% H]".
+  iExists e2; iSplit; first done. iIntros "!>".
+  iApply (wp_strong_mono with "H").
   iIntros (v) "H". by iApply "H".
 Qed.
 
-Lemma wp_bind K `{!LanguageCtx K} s E e Φ :
-  WP e @ s; E {{ v, WP K (of_val v) @ s; E {{ Φ }} }} ⊢ WP K e @ s; E {{ Φ }}.
+Lemma wp_bind K `{!LanguageCtx K} e Φ :
+  WP e {{ v, WP K (of_val v) {{ Φ }} }} ⊢ WP K e {{ Φ }}.
 Proof.
-  iIntros "H". iLöb as "IH" forall (E e Φ). rewrite wp_unfold /wp_pre.
-  destruct (to_val e) as [v|] eqn:He.
-  { by apply of_to_val in He as <-. }
+  iIntros "H". iLöb as "IH" forall (e Φ). rewrite wp_unfold /wp_pre.
+  destruct (to_val e) as [v|] eqn:He; first by apply of_to_val in He as <-.
   rewrite wp_unfold /wp_pre fill_not_val //.
-  iIntros (σ1 κ κs n) "Hσ". iDestruct ("H" with "[$]") as "[% H]".
-  iSplit.
-  { iPureIntro. destruct s; last done.
-    unfold reducible in *. naive_solver eauto using fill_step. }
-  iIntros (e2 σ2 efs Hstep).
-  destruct (fill_step_inv e σ1 κ e2 σ2 efs) as (e2'&->&?); auto.
-  iDestruct ("H" $! e2' σ2 efs with "[//]") as "H". iIntros "!>".
-  iDestruct "H" as "(Hσ & H & Hefs)".
-  iFrame "Hσ Hefs". by iApply "IH".
+  iDestruct "H" as (e2 ?) "H"; iExists (K e2); iSplit; last by iApply "IH".
+  iPureIntro. exact: fill_step.
 Qed.
 
-Lemma wp_bind_inv K `{!LanguageCtx K} s E e Φ :
-  WP K e @ s; E {{ Φ }} ⊢ WP e @ s; E {{ v, WP K (of_val v) @ s; E {{ Φ }} }}.
+Lemma wp_bind_inv K `{!LanguageCtx K} e Φ :
+  WP K e {{ Φ }} ⊢ WP e {{ v, WP K (of_val v) {{ Φ }} }}.
 Proof.
-  iIntros "H". iLöb as "IH" forall (E e Φ). rewrite !wp_unfold /wp_pre.
+  iIntros "H". iLöb as "IH" forall (e Φ). rewrite !wp_unfold /wp_pre.
   destruct (to_val e) as [v|] eqn:He.
   { apply of_to_val in He as <-. by rewrite !wp_unfold /wp_pre. }
   rewrite fill_not_val //.
-  iIntros (σ1 κ κs n) "Hσ". iDestruct ("H" with "[$]") as "[% H]". iSplit.
-  { destruct s; eauto using reducible_fill. }
-  iIntros (e2 σ2 efs Hstep).
-  iDestruct ("H" $! (K e2) σ2 efs with "[]") as "H"; [by eauto using fill_step|].
-  iIntros "!>". iDestruct "H" as "(Hσ & H & Hefs)".
-  iFrame "Hσ Hefs". by iApply "IH".
+  iDestruct "H" as (eK2 Hkstep) "H".
+  edestruct (fill_step_inv e) with (e2 := eK2) as (e2 & -> & ?) => //.
+  iExists e2; iSplit; first done. by iApply "IH".
 Qed.
 
 (** * Derived rules *)
-Lemma wp_mono s E e Φ Ψ : (∀ v, Φ v ⊢ Ψ v) → WP e @ s; E {{ Φ }} ⊢ WP e @ s; E {{ Ψ }}.
+Lemma wp_mono e Φ Ψ : (∀ v, Φ v ⊢ Ψ v) → WP e {{ Φ }} ⊢ WP e {{ Ψ }}.
 Proof.
   iIntros (HΦ) "H"; iApply (wp_strong_mono with "H"); auto.
   iIntros (v) "?". by iApply HΦ.
 Qed.
-Global Instance wp_mono' s E e :
-  Proper (pointwise_relation _ (⊢) ==> (⊢)) (wp (PROP:=iProp Σ) s E e).
-Proof. by intros Φ Φ' ?; apply wp_mono. Qed.
+Global Instance wp_mono' e :
+  Proper (pointwise_relation _ (⊢) ==> (⊢)) (wp (PROP:=iProp Σ) NotStuck ⊤ e).
+Proof. intros Φ Φ' ?. by apply wp_mono. Qed.
 
-Lemma wp_value s E Φ e v : IntoVal e v → Φ v ⊢ WP e @ s; E {{ Φ }}.
+Lemma wp_value Φ e v : IntoVal e v → Φ v ⊢ WP e {{ Φ }}.
 Proof. intros <-. by apply wp_value'. Qed.
-Lemma wp_value_inv s E Φ e v : IntoVal e v → WP e @ s; E {{ Φ }} ⊢ Φ v.
+Lemma wp_value_inv Φ e v : IntoVal e v → WP e {{ Φ }} ⊢ Φ v.
 Proof. intros <-. by apply wp_value_inv'. Qed.
 
-Lemma wp_frame_l s E e Φ R : R ∗ WP e @ s; E {{ Φ }} ⊢ WP e @ s; E {{ v, R ∗ Φ v }}.
+Lemma wp_frame_l e Φ R : R ∗ WP e {{ Φ }} ⊢ WP e {{ v, R ∗ Φ v }}.
 Proof. iIntros "[? H]". iApply (wp_strong_mono with "H"); auto with iFrame. Qed.
-Lemma wp_frame_r s E e Φ R : WP e @ s; E {{ Φ }} ∗ R ⊢ WP e @ s; E {{ v, Φ v ∗ R }}.
+Lemma wp_frame_r e Φ R : WP e {{ Φ }} ∗ R ⊢ WP e {{ v, Φ v ∗ R }}.
 Proof. iIntros "[H ?]". iApply (wp_strong_mono with "H"); auto with iFrame. Qed.
 
-Lemma wp_frame_step_l s E1 E2 e Φ R :
+Lemma wp_frame_step_l e Φ R :
   to_val e = None →
-  (▷R) ∗ WP e @ s; E2 {{ Φ }} ⊢ WP e @ s; E1 {{ v, R ∗ Φ v }}.
+  (▷R) ∗ WP e {{ Φ }} ⊢ WP e {{ v, R ∗ Φ v }}.
 Proof.
   iIntros (?) "[Hu Hwp]". iApply (wp_step with "Hu"); try done.
   iApply (wp_mono with "Hwp"). by iIntros (?) "$$".
 Qed.
-Lemma wp_frame_step_r s E1 E2 e Φ R :
+Lemma wp_frame_step_r e Φ R :
   to_val e = None →
-  WP e @ s; E2 {{ Φ }} ∗ (▷R) ⊢ WP e @ s; E1 {{ v, Φ v ∗ R }}.
+  WP e {{ Φ }} ∗ (▷R) ⊢ WP e {{ v, Φ v ∗ R }}.
 Proof.
   rewrite [(WP _ @ _; _ {{ _ }} ∗ _)%I]comm; setoid_rewrite (comm _ _ R).
   apply wp_frame_step_l.
 Qed.
-Lemma wp_frame_step_l' s E e Φ R :
-  to_val e = None → ▷ R ∗ WP e @ s; E {{ Φ }} ⊢ WP e @ s; E {{ v, R ∗ Φ v }}.
-Proof. iIntros (?) "[??]". iApply (wp_frame_step_l s E E); try iFrame; eauto. Qed.
-Lemma wp_frame_step_r' s E e Φ R :
-  to_val e = None → WP e @ s; E {{ Φ }} ∗ ▷ R ⊢ WP e @ s; E {{ v, Φ v ∗ R }}.
-Proof. iIntros (?) "[??]". iApply (wp_frame_step_r s E E); try iFrame; eauto. Qed.
+Lemma wp_frame_step_l' e Φ R :
+  to_val e = None → ▷ R ∗ WP e {{ Φ }} ⊢ WP e {{ v, R ∗ Φ v }}.
+Proof. iIntros (?) "[??]". iApply wp_frame_step_l; try iFrame; eauto. Qed.
+Lemma wp_frame_step_r' e Φ R :
+  to_val e = None → WP e {{ Φ }} ∗ ▷ R ⊢ WP e {{ v, Φ v ∗ R }}.
+Proof. iIntros (?) "[??]". iApply wp_frame_step_r; try iFrame; eauto. Qed.
 
-Lemma wp_wand s E e Φ Ψ :
-  WP e @ s; E {{ Φ }} -∗ (∀ v, Φ v -∗ Ψ v) -∗ WP e @ s; E {{ Ψ }}.
+Lemma wp_wand e Φ Ψ :
+  WP e {{ Φ }} -∗ (∀ v, Φ v -∗ Ψ v) -∗ WP e {{ Ψ }}.
 Proof.
   iIntros "Hwp H". iApply (wp_strong_mono with "Hwp"); auto.
 Qed.
-Lemma wp_wand_l s E e Φ Ψ :
-  (∀ v, Φ v -∗ Ψ v) ∗ WP e @ s; E {{ Φ }} ⊢ WP e @ s; E {{ Ψ }}.
+Lemma wp_wand_l e Φ Ψ :
+  (∀ v, Φ v -∗ Ψ v) ∗ WP e {{ Φ }} ⊢ WP e {{ Ψ }}.
 Proof. iIntros "[H Hwp]". iApply (wp_wand with "Hwp H"). Qed.
-Lemma wp_wand_r s E e Φ Ψ :
-  WP e @ s; E {{ Φ }} ∗ (∀ v, Φ v -∗ Ψ v) ⊢ WP e @ s; E {{ Ψ }}.
+Lemma wp_wand_r e Φ Ψ :
+  WP e {{ Φ }} ∗ (∀ v, Φ v -∗ Ψ v) ⊢ WP e {{ Ψ }}.
 Proof. iIntros "[Hwp H]". iApply (wp_wand with "Hwp H"). Qed.
 End wp.
 
@@ -216,8 +191,8 @@ Section proofmode_classes.
   Implicit Types P Q : iProp Σ.
   Implicit Types Φ : val Λ → iProp Σ.
 
-  Global Instance frame_wp p s E e R Φ Ψ :
+  Global Instance frame_wp p e R Φ Ψ :
     (∀ v, Frame p R (Φ v) (Ψ v)) →
-    Frame p R (WP e @ s; E {{ Φ }}) (WP e @ s; E {{ Ψ }}).
+    Frame p R (WP e {{ Φ }}) (WP e {{ Ψ }}).
   Proof. rewrite /Frame=> HR. rewrite wp_frame_l. apply wp_mono, HR. Qed.
 End proofmode_classes.
